Equivalence checking for i2c

i2c/i2c_wrapper.sv
@@ -1,0 +1,72 @@
+typedef struct packed {
+  logic [47:0] addr;
+  logic write;
+  logic [31:0] wdata;
+  logic [3:0] wstrb;
+  logic valid;
+} reg_req_t;
+
+typedef struct packed {
+  logic [31:0] rdata;
+  logic error;
+  logic ready;
+} reg_rsp_t;
+
+module i2c_circuit (
+  input logic clk_i,
+  input logic rst_ni,
+  input logic [85:0] reg_req_i,
+  input logic cio_scl_i,
+  input logic cio_sda_i,
+  output logic [33:0] reg_rsp_o,
+  output logic cio_scl_o,
+  output logic cio_scl_en_o,
+  output logic cio_sda_o,
+  output logic cio_sda_en_o,
+  output logic intr_fmt_threshold_o,
+  output logic intr_rx_threshold_o,
+  output logic intr_fmt_overflow_o,
+  output logic intr_rx_overflow_o,
+  output logic intr_nak_o,
+  output logic intr_scl_interference_o,
+  output logic intr_sda_interference_o,
+  output logic intr_stretch_timeout_o,
+  output logic intr_sda_unstable_o,
+  output logic intr_cmd_complete_o,
+  output logic intr_tx_stretch_o,
+  output logic intr_tx_overflow_o,
+  output logic intr_acq_full_o,
+  output logic intr_unexp_stop_o,
+  output logic intr_host_timeout_o
+);
+  i2c #(
+    .reg_req_t(reg_req_t),
+    .reg_rsp_t(reg_rsp_t)
+  ) inner (
+    .clk_i,
+    .rst_ni,
+    .reg_req_i,
+    .cio_scl_i,
+    .cio_sda_i,
+    .reg_rsp_o,
+    .cio_scl_o,
+    .cio_scl_en_o,
+    .cio_sda_o,
+    .cio_sda_en_o,
+    .intr_fmt_threshold_o,
+    .intr_rx_threshold_o,
+    .intr_fmt_overflow_o,
+    .intr_rx_overflow_o,
+    .intr_nak_o,
+    .intr_scl_interference_o,
+    .intr_sda_interference_o,
+    .intr_stretch_timeout_o,
+    .intr_sda_unstable_o,
+    .intr_cmd_complete_o,
+    .intr_tx_stretch_o,
+    .intr_tx_overflow_o,
+    .intr_acq_full_o,
+    .intr_unexp_stop_o,
+    .intr_host_timeout_o
+  );
+endmodule
